rt refine: sorry rest of Refine session
Signed-off-by: Gerwin Klein <gerwin.klein@data61.csiro.au>

proof/refine/ARM/DomainTime_R.thy
@@ -15,10 +15,6 @@ text \<open>Preservation of domain time remaining over kernel invocations;
 
 context begin interpretation Arch . (*FIXME: arch_split*)
 
-(* FIXME move to DetSchedDomainTime_AI *)
-crunch domain_list_inv[wp]: do_user_op "\<lambda>s. P (domain_list s)"
-  (wp: select_wp)
-
 (* abstract and haskell have identical domain list fields *)
 abbreviation
   valid_domain_list' :: "'a kernel_state_scheme \<Rightarrow> bool"
@@ -32,7 +28,7 @@ lemmas valid_domain_list'_def = valid_domain_list_2_def
 crunches sendFaultIPC, handleFault, replyFromKernel, setDomain, sendSignal,
          finaliseCap, finaliseCap, capSwapForDelete
   for ksDomSchedule_inv[wp]: "\<lambda>s. P (ksDomSchedule s)"
-  (wp: getObject_inv loadObject_default_inv crunch_wps
+  (wp: getObject_inv loadObject_default_inv crunch_wps hoare_vcg_all_lift whileM_inv
    simp: crunch_simps if_apply_def2 unless_def o_def assertE_def)
 
 lemma finaliseSlot_ksDomSchedule_inv[wp]:
@@ -43,14 +39,9 @@ crunch ksDomSchedule_inv[wp]: invokeTCB "\<lambda>s. P (ksDomSchedule s)"
   (wp: crunch_wps checkCap_inv finaliseSlot'_preservation simp: if_apply_def2 crunch_simps)
 
 crunch ksDomSchedule_inv[wp]: doReplyTransfer "\<lambda>s. P (ksDomSchedule s)"
-  (wp: crunch_wps transferCapsToSlots_pres1 setObject_ep_ct
-       setObject_ntfn_ct
+  (wp: crunch_wps transferCapsToSlots_pres1
    simp: unless_def crunch_simps
    ignore: transferCapsToSlots)
-
-crunch ksDomSchedule_inv[wp]: finaliseCap "\<lambda>s. P (ksDomSchedule s)"
-  (simp: crunch_simps assertE_def unless_def
-     wp: getObject_inv loadObject_default_inv crunch_wps)
 
 crunch ksDomSchedule_inv[wp]: cancelBadgedSends "\<lambda>s. P (ksDomSchedule s)"
   (simp: filterM_mapM crunch_simps
@@ -67,29 +58,31 @@ crunch ksDomSchedule_inv[wp]: performARMMMUInvocation "\<lambda>s. P (ksDomSched
    simp: unless_def)
 
 crunch ksDomSchedule_inv[wp]: performInvocation "\<lambda>s. P (ksDomSchedule s)"
-  (wp: crunch_wps zipWithM_x_inv cteRevoke_preservation mapME_x_inv_wp
+  (wp: crunch_wps zipWithM_x_inv cteRevoke_preservation mapME_x_inv_wp hoare_vcg_all_lift
    simp: unless_def crunch_simps filterM_mapM)
 
 crunch ksDomSchedule_inv[wp]: schedule "\<lambda>s. P (ksDomSchedule s)"
-  (ignore: setNextPC threadSet simp: crunch_simps bitmap_fun_defs wp:findM_inv hoare_drop_imps)
+  (ignore: setNextPC threadSet simp: crunch_simps bitmap_fun_defs
+   wp: whileM_inv findM_inv hoare_drop_imps)
 
 crunch ksDomSchedule_inv[wp]: activateThread "\<lambda>s. P (ksDomSchedule s)"
+  (simp: crunch_simps wp: crunch_wps)
 
-crunches receiveSignal, getNotification, receiveIPC, deleteCallerCap
+crunches receiveSignal, getNotification, receiveIPC, lookupReply, mcsIRQ
   for ksDomSchedule_inv[wp]: "\<lambda>s. P (ksDomSchedule s)"
   (wp: hoare_drop_imps simp: crunch_simps)
 
 lemma handleRecv_ksDomSchedule_inv[wp]:
-  "\<lbrace>\<lambda>s. P (ksDomSchedule s) \<rbrace> handleRecv e \<lbrace>\<lambda>_ s. P (ksDomSchedule s) \<rbrace>"
+  "\<lbrace>\<lambda>s. P (ksDomSchedule s) \<rbrace> handleRecv b e \<lbrace>\<lambda>_ s. P (ksDomSchedule s) \<rbrace>"
   unfolding handleRecv_def
   by (rule hoare_pre)
-     (wp hoare_drop_imps | simp add: crunch_simps | wpc)+
+     (wp hoare_drop_imps | simp add: crunch_simps split del: if_split | wpc)+
 
 context
 notes if_cong [cong]
 begin
 crunch ksDomSchedule_inv[wp]: handleEvent "\<lambda>s. P (ksDomSchedule s)"
-  (wp: syscall_valid' ignore: syscall)
+  (wp: syscall_valid' crunch_wps ignore: syscall)
 end
 
 lemma callKernel_ksDomSchedule_inv[wp]:
@@ -107,23 +100,19 @@ crunches setExtraBadge, cteInsert
 
 crunch ksDomainTime[wp]: transferCapsToSlots "\<lambda>s. P (ksDomainTime s)"
 
-crunches  setupCallerCap, doIPCTransfer, possibleSwitchTo
+crunches doIPCTransfer, possibleSwitchTo
   for ksDomainTime[wp]: "\<lambda>s. P (ksDomainTime s)"
   (wp: crunch_wps simp: zipWithM_x_mapM ignore: constOnFailure)
 
-crunches setEndpoint, setNotification, storePTE, storePDE
-  for ksDomainTime_inv[wp]:
-  "\<lambda>s. P (ksDomainTime s)"
-  (wp: crunch_wps setObject_ksPSpace_only updateObject_default_inv)
-
 crunches sendFaultIPC, handleFault, replyFromKernel
   for ksDomainTime_inv[wp]: "\<lambda>s. P (ksDomainTime s)"
+  (wp: crunch_wps whileM_inv hoare_vcg_all_lift simp: crunch_simps)
 
 crunch ksDomainTime_inv[wp]: setDomain "\<lambda>s. P (ksDomainTime s)"
   (wp: crunch_wps simp: if_apply_def2)
 
 crunch ksDomainTime_inv[wp]: sendSignal "\<lambda>s. P (ksDomainTime s)"
-  (wp: crunch_wps simp: crunch_simps simp: unless_def o_def)
+  (wp: crunch_wps gts_wp' simp: crunch_simps simp: unless_def o_def)
 
 crunch ksDomainTime_inv[wp]: deleteASID "\<lambda>s. P (ksDomainTime s)"
   (wp: crunch_wps setObject_ksPSpace_only getObject_inv loadObject_default_inv
@@ -132,7 +121,7 @@ crunch ksDomainTime_inv[wp]: deleteASID "\<lambda>s. P (ksDomainTime s)"
 
 crunch ksDomainTime_inv[wp]: finaliseCap "\<lambda>s. P (ksDomainTime s)"
   (simp: crunch_simps assertE_def
-     wp: setObject_ksPSpace_only getObject_inv loadObject_default_inv crunch_wps)
+     wp: setObject_ksPSpace_only getObject_inv loadObject_default_inv crunch_wps hoare_vcg_all_lift)
 
 crunch ksDomainTime_inv[wp]: cancelBadgedSends "\<lambda>s. P (ksDomainTime s)"
   (wp: crunch_wps setObject_ksPSpace_only getObject_inv loadObject_default_inv
@@ -150,18 +139,9 @@ crunch ksDomainTime_inv[wp]: invokeTCB "\<lambda>s. P (ksDomainTime s)"
   (wp: crunch_wps checkCap_inv finaliseSlot'_preservation simp: if_apply_def2 crunch_simps)
 
 crunch ksDomainTime_inv[wp]: doReplyTransfer "\<lambda>s. P (ksDomainTime s)"
-  (wp: crunch_wps transferCapsToSlots_pres1 setObject_ep_ct
-       setObject_ntfn_ct
+  (wp: crunch_wps transferCapsToSlots_pres1
    simp: crunch_simps
    ignore: transferCapsToSlots)
-
-crunch ksDomainTime_inv[wp]: finaliseCap "\<lambda>s. P (ksDomainTime s)"
-  (simp: crunch_simps assertE_def unless_def
-     wp: getObject_inv loadObject_default_inv crunch_wps)
-
-crunch ksDomainTime_inv[wp]: cancelBadgedSends "\<lambda>s. P (ksDomainTime s)"
-  (simp: filterM_mapM crunch_simps
-     wp: crunch_wps)
 
 crunch ksDomainTime_inv[wp]: createNewObjects "\<lambda>s. P (ksDomainTime s)"
   (simp: crunch_simps zipWithM_x_mapM
@@ -174,27 +154,31 @@ crunch ksDomainTime_inv[wp]: performARMMMUInvocation "\<lambda>s. P (ksDomainTim
 crunch ksDomainTime_inv[wp]: preemptionPoint "\<lambda>s. P (ksDomainTime s)"
   (simp: whenE_def ignore_del: preemptionPoint)
 
-crunch ksDomainTime_inv[wp]: performInvocation "\<lambda>s. P (ksDomainTime s)"
-  (wp: crunch_wps zipWithM_x_inv cteRevoke_preservation mapME_x_inv_wp
+crunches activateThread, lookupReply
+  for ksDomainTime_inv[wp]: "\<lambda>s. P (ksDomainTime s)"
+  (wp: crunch_wps)
+
+(* Does not hold for all of performInvocation (invokeSchedControlConfigure) *)
+crunches invokeUntyped, invokeSchedContext, invokeCNode, performIRQControl, invokeIRQHandler
+  for ksDomainTime_inv[wp]:  "\<lambda>s. P (ksDomainTime s)"
+  (wp: crunch_wps zipWithM_x_inv cteRevoke_preservation mapME_x_inv_wp hoare_vcg_all_lift
    simp: unless_def crunch_simps filterM_mapM)
 
-crunch ksDomainTime_inv[wp]: activateThread "\<lambda>s. P (ksDomainTime s)"
-
-crunches receiveSignal, getNotification, receiveIPC, deleteCallerCap
+crunches receiveSignal, getNotification, receiveIPC
   for ksDomainTime_inv[wp]: "\<lambda>s. P (ksDomainTime s)"
   (wp: hoare_drop_imps simp: crunch_simps)
 
 lemma handleRecv_ksDomainTime_inv[wp]:
-  "\<lbrace>\<lambda>s. P (ksDomainTime s) \<rbrace> handleRecv e \<lbrace>\<lambda>_ s. P (ksDomainTime s) \<rbrace>"
+  "\<lbrace>\<lambda>s. P (ksDomainTime s) \<rbrace> handleRecv b e \<lbrace>\<lambda>_ s. P (ksDomainTime s) \<rbrace>"
   unfolding handleRecv_def
   by (rule hoare_pre)
-     (wp hoare_drop_imps | simp add: crunch_simps | wpc)+
+     (wp hoare_drop_imps | simp add: crunch_simps split del: if_split | wpc)+
 
 crunches doUserOp, getIRQState, chooseThread, handleYield
   for ksDomainTime_inv[wp]: "(\<lambda>s. P (ksDomainTime s))"
-  (wp: select_wp)
+  (wp: crunch_wps select_wp)
 
-crunches handleSend, handleReply, handleCall, handleHypervisorFault
+crunches handleHypervisorFault
   for ksDomainTime_inv[wp]: "(\<lambda>s. P (ksDomainTime s))"
   (wp: syscall_valid' ignore: syscall)
 
@@ -206,28 +190,17 @@ lemma nextDomain_domain_time_left'[wp]:
    apply (wpsimp simp: valid_domain_list'_def dschLength_def)
    apply (simp only: all_set_conv_all_nth)
    apply (erule_tac x="Suc (ksDomScheduleIdx s) mod length (ksDomSchedule s)" in allE)
-   apply fastforce
-   done
+   apply clarsimp
+   sorry (* FIXME RT: not true, need overflow protection in valid_domain_list_2. Also usToMs should be ms_to_us *)
 
-lemma rescheduleRequired_ksSchedulerAction[wp]:
-  "\<lbrace>\<top>\<rbrace> rescheduleRequired \<lbrace>\<lambda>_ s. ksSchedulerAction s = ChooseNewThread \<rbrace>"
-  unfolding rescheduleRequired_def
-  by (wp setSchedulerAction_direct)
-
-lemma timerTick_valid_domain_time:
-  "\<lbrace>\<lambda>s. 0 < ksDomainTime s\<rbrace>
-   timerTick
-   \<lbrace>\<lambda>_ s. ksDomainTime s = 0 \<longrightarrow> ksSchedulerAction s = ChooseNewThread\<rbrace>"
-  apply (simp add: timerTick_def numDomains_def)
-  apply wp
-       apply (rule_tac Q="\<lambda>_ s. ksSchedulerAction s = ChooseNewThread" in hoare_strengthen_post)
-        apply (wp | clarsimp simp: if_apply_def2)+
-  done
+(* if domain time is up, scheduler must run *)
+abbreviation domain_time_sched :: "kernel_state \<Rightarrow> bool" where
+  "domain_time_sched s \<equiv> ksDomainTime s = 0 \<longrightarrow> ksSchedulerAction s = ChooseNewThread"
 
 lemma handleInterrupt_valid_domain_time:
   "\<lbrace>\<lambda>s.  0 < ksDomainTime s \<rbrace>
    handleInterrupt i
-   \<lbrace>\<lambda>rv s.  ksDomainTime s = 0 \<longrightarrow> ksSchedulerAction s = ChooseNewThread\<rbrace>"
+   \<lbrace>\<lambda>_.  domain_time_sched\<rbrace>"
    apply (simp add: handleInterrupt_def)
    apply (case_tac "maxIRQ < i"; simp)
     subgoal by (wp hoare_false_imp) simp
@@ -241,22 +214,34 @@ lemma handleInterrupt_valid_domain_time:
      apply (rule_tac Q="\<lambda>_ s. 0 < ksDomainTime s" in hoare_post_imp, clarsimp)
      apply wp
     (* IRQTimer : tick occurs *) (* IRQReserved : trivial *)
-    apply (wp timerTick_valid_domain_time
-          | clarsimp simp: handleReservedIRQ_def
+    apply (wp
+          | clarsimp simp: handleReservedIRQ_def setReprogramTimer_def
           | wp (once) hoare_vcg_imp_lift)+
   done
 
+crunches setNextInterrupt, getReprogramTimer
+  for ksDomainTime_inv[wp]:  "\<lambda>s. P (ksDomainTime s)"
+  (wp: crunch_wps
+   simp: crunch_simps)
+
+lemma scheduleChooseNewThread_domainTime[wp]:
+  "\<lbrace> valid_domain_list' \<rbrace>
+   scheduleChooseNewThread
+   \<lbrace>\<lambda>_ s. 0 < ksDomainTime s \<rbrace>"
+  unfolding scheduleChooseNewThread_def
+  by (wpsimp simp: word_neq_0_conv)
+
 lemma schedule_domain_time_left':
-  "\<lbrace> valid_domain_list' and
-     (\<lambda>s. ksDomainTime s = 0 \<longrightarrow> ksSchedulerAction s = ChooseNewThread) \<rbrace>
+  "\<lbrace> valid_domain_list' and domain_time_sched \<rbrace>
    ThreadDecls_H.schedule
    \<lbrace>\<lambda>_ s. 0 < ksDomainTime s \<rbrace>"
-  unfolding schedule_def scheduleChooseNewThread_def
-  supply word_neq_0_conv[simp]
-  apply wpsimp+
+  unfolding schedule_def
+  apply wpsimp
+  sorry (* FIXME RT: this might need code change
+  apply (wpsimp wp: threadGet_wp)
        apply (rule_tac Q="\<lambda>_. valid_domain_list'" in hoare_post_imp, clarsimp)
        apply (wp | clarsimp | wp (once) hoare_drop_imps)+
-  done
+  done *)
 
 lemma handleEvent_ksDomainTime_inv:
   "\<lbrace>\<lambda>s. P (ksDomainTime  s) \<and> e \<noteq> Interrupt \<rbrace>
@@ -266,7 +251,7 @@ lemma handleEvent_ksDomainTime_inv:
       apply (rename_tac syscall)
       apply (case_tac syscall, simp_all add: handle_send_def)
              apply (wp hv_inv'|simp add: handleEvent_def cong: if_cong|wpc)+
-  done
+  sorry (* FIXME RT: needs rephrasing or code change for invokeSchedControl *)
 
 lemma callKernel_domain_time_left:
   "\<lbrace> (\<lambda>s. 0 < ksDomainTime s) and valid_domain_list' and (\<lambda>s. e \<noteq> Interrupt \<longrightarrow> ct_running' s) \<rbrace>
@@ -282,6 +267,7 @@ lemma callKernel_domain_time_left:
           | wpc | simp)+)[1]
     apply (rule_tac Q="\<lambda>_ s. 0 < ksDomainTime s \<and> valid_domain_list' s" in hoare_post_imp)
      apply fastforce
+  sorry (*
     apply wp
    apply simp
   (* non-interrupt case; may throw but does not touch ksDomainTime in handleEvent *)
@@ -296,7 +282,7 @@ lemma callKernel_domain_time_left:
    apply (rule_tac Q="\<lambda>_ s. valid_domain_list' s \<and> 0 < ksDomainTime s"
             in NonDetMonadVCG.hoare_post_impErr[rotated 2], assumption)
     apply (wp handleEvent_ksDomainTime_inv | clarsimp)+
-  done
+  done *)
 
 end
 
