proof/refine/ARM/PageTableDuplicates.thy
@@ -62,7 +62,7 @@ lemma setCTE_valid_duplicates'[wp]:
      apply (erule valid_duplicates'_non_pd_pt_I[rotated 3],simp+)+
   done
 
-crunches cteInsert, setupReplyMaster
+crunches cteInsert
   for valid_duplicates'[wp]: "(\<lambda>s. vs_valid_duplicates' (ksPSpace s))"
   (wp: crunch_wps simp: crunch_simps)
 
@@ -72,7 +72,7 @@ lemma doMachineOp_ksPSpace_inv[wp]:
 
 crunches threadSet, setBoundNotification, setExtraBadge
   for valid_duplicates'[wp]: "\<lambda>s. vs_valid_duplicates' (ksPSpace s)"
-  (wp: setObject_ksInterrupt updateObject_default_inv)
+  (wp: updateObject_default_inv)
 
 lemma transferCapsToSlots_duplicates'[wp]:
  "\<lbrace>\<lambda>s. vs_valid_duplicates' (ksPSpace s)\<rbrace>
@@ -80,11 +80,39 @@ lemma transferCapsToSlots_duplicates'[wp]:
   \<lbrace>\<lambda>rv s. vs_valid_duplicates' (ksPSpace s)\<rbrace>"
   by (rule transferCapsToSlots_pres1; wp)
 
+lemma setObjectSC_valid_duplicates'[wp]:
+  "setObject a (sc::sched_context) \<lbrace>\<lambda>s. vs_valid_duplicates' (ksPSpace s)\<rbrace>"
+  apply (clarsimp simp: setObject_def split_def valid_def in_monad
+                        projectKOs pspace_aligned'_def ps_clear_upd'
+                        objBits_def[symmetric] lookupAround2_char1
+                 split: if_split_asm)
+  apply (frule pspace_storable_class.updateObject_type[where v = sc,simplified])
+  apply (clarsimp simp: updateObject_default_def assert_def bind_def
+                        alignCheck_def in_monad when_def alignError_def magnitudeCheck_def
+                        assert_opt_def return_def fail_def typeError_def
+                  split: if_splits option.splits Structures_H.kernel_object.splits)
+     apply (erule valid_duplicates'_non_pd_pt_I[rotated 3],simp+)+
+  done
+
+lemma setObjectReply_valid_duplicates'[wp]:
+  "setObject a (r::reply) \<lbrace>\<lambda>s. vs_valid_duplicates' (ksPSpace s)\<rbrace>"
+  apply (clarsimp simp: setObject_def split_def valid_def in_monad
+                        projectKOs pspace_aligned'_def ps_clear_upd'
+                        objBits_def[symmetric] lookupAround2_char1
+                 split: if_split_asm)
+  apply (frule pspace_storable_class.updateObject_type[where v = r,simplified])
+  apply (clarsimp simp: updateObject_default_def assert_def bind_def
+                        alignCheck_def in_monad when_def alignError_def magnitudeCheck_def
+                        assert_opt_def return_def fail_def typeError_def
+                  split: if_splits option.splits Structures_H.kernel_object.splits)
+     apply (erule valid_duplicates'_non_pd_pt_I[rotated 3],simp+)+
+  done
+
 crunches transferCaps, sendFaultIPC, handleFault, replyFromKernel, insertNewCap
   for valid_duplicates'[wp]: "\<lambda>s. vs_valid_duplicates' (ksPSpace s)"
   (ignore: transferCapsToSlots
-       wp: crunch_wps hoare_vcg_const_Ball_lift get_rs_cte_at'
-     simp: zipWithM_x_mapM ball_conj_distrib)
+       wp: crunch_wps hoare_vcg_const_Ball_lift hoare_vcg_all_lift get_rs_cte_at' whileM_inv
+     simp: zipWithM_x_mapM ball_conj_distrib crunch_simps)
 
 lemma koTypeOf_pte:
   "koTypeOf ko = ArchT PTET \<Longrightarrow> \<exists>pte. ko = KOArch (KOPTE pte)"
@@ -110,15 +138,13 @@ lemma mapM_x_storePTE_updates:
   apply clarsimp
   apply (intro conjI ballI)
    apply (drule(1) bspec)
-   apply (clarsimp simp:typ_at'_def ko_wp_at'_def
-     objBits_simps archObjSize_def dest!:koTypeOf_pte
-     split:  Structures_H.kernel_object.split_asm)
+   apply (clarsimp simp: typ_at'_def ko_wp_at'_def objBits_defs
+                   dest!: koTypeOf_pte
+                   split:  kernel_object.split_asm)
    apply (simp add:ps_clear_def dom_fun_upd2[unfolded fun_upd_def])
+   apply (simp add: lookupAround2_known1)
   apply (erule rsubst[where P=Q])
   apply (rule ext, clarsimp)
-  apply (case_tac "(fst (lookupAround2 aa (ksPSpace s)))")
-   apply (clarsimp simp:lookupAround2_None1)
-  apply (clarsimp simp:lookupAround2_known1)
   done
 
 lemma is_aligned_plus_bound:
@@ -350,6 +376,7 @@ lemma mapM_x_storePTE_update_helper:
       apply (simp add:objBits_simps' archObjSize_def pteBits_def
         is_aligned_weaken[where y = 2] pageBits_def pdeBits_def
         split:kernel_object.splits arch_kernel_object.splits)
+  sorry (*
      apply (simp add:mask_lower_twice)
      apply (drule mask_out_first_mask_some[where m = ptBits])
       apply (simp add:vs_ptr_align_def
@@ -376,7 +403,7 @@ lemma mapM_x_storePTE_update_helper:
   apply (clarsimp split:option.splits)
   apply (drule_tac p' = y in valid_duplicates'_D)
      apply simp+
-  done
+  done *)
 
 lemma page_directory_at_pde_atD':
   "\<lbrakk>page_directory_at' p s;is_aligned p' 2; p' && ~~ mask pdBits = p\<rbrakk> \<Longrightarrow> pde_at' p' s"
@@ -413,12 +440,13 @@ lemma mapM_x_storePDE_updates:
      objBits_simps archObjSize_def dest!:koTypeOf_pde
      split:  Structures_H.kernel_object.split_asm  arch_kernel_object.split_asm if_split)
    apply (simp add:ps_clear_def dom_fun_upd2[unfolded fun_upd_def])
+  sorry (*
   apply (erule rsubst[where P=Q])
   apply (rule ext, clarsimp)
   apply (case_tac "(fst (lookupAround2 aa (ksPSpace s)))")
    apply (clarsimp simp:lookupAround2_None1)
   apply (clarsimp simp:lookupAround2_known1)
-  done
+  done *)
 
 lemma mapM_x_storePDE_update_helper:
   "\<lbrace>\<lambda>s. vs_valid_duplicates' (ksPSpace s)
@@ -465,6 +493,7 @@ lemma mapM_x_storePDE_update_helper:
       apply (simp add:objBits_simps' archObjSize_def pteBits_def
         is_aligned_weaken[where y = 2] pageBits_def pdeBits_def
         split:kernel_object.splits arch_kernel_object.splits)
+  sorry (*
      apply (simp add:mask_lower_twice)
      apply (drule mask_out_first_mask_some[where m = pdBits])
       apply (simp add:vs_ptr_align_def
@@ -491,7 +520,7 @@ lemma mapM_x_storePDE_update_helper:
   apply (clarsimp split:option.splits)
   apply (drule_tac p' = y in valid_duplicates'_D)
      apply simp+
-  done
+  done *)
 
 lemma vs_ptr_align_upbound:
   "vs_ptr_align a \<le> 6"
@@ -589,7 +618,7 @@ lemma copyGlobalMappings_ksPSpace_stable:
       apply (simp add: archObjSize_def pageBits_def
                        pteBits_def pdeBits_def
                   split: arch_kernel_object.splits)
-      done
+      sorry
     have ptr_eqD:
       "\<And>p a b. \<lbrakk>p + a = ptr + b;is_aligned p pdBits;
             a < 2^ pdBits; b < 2^pdBits \<rbrakk>
@@ -703,6 +732,7 @@ lemma copyGlobalMappings_ksPSpace_stable:
         | simp add: storePDE_def setObject_def split_def
         updateObject_default_def
         split: option.splits)+
+  sorry (*
      apply (clarsimp simp:objBits_simps archObjSize_def)
      apply (clarsimp simp:obj_at'_def objBits_simps
         projectKO_def projectKO_opt_pde fail_def return_def
@@ -741,7 +771,7 @@ lemma copyGlobalMappings_ksPSpace_stable:
     apply (clarsimp simp:objBits_simps archObjSize_def pdeBits_def dest!:in_rangeD)
    apply wp
   apply simp
-  done
+  done *)
 qed
 
 lemma copyGlobalMappings_ksPSpace_same:
@@ -1158,8 +1188,7 @@ lemma createObject_valid_duplicates'[wp]:
   apply (clarsimp simp: word_bits_def)
   apply (drule_tac ptr = ptr and ko = "KOCTE makeObject" in
     valid_duplicates'_insert_ko[where us = us,simplified])
-      apply (simp add: APIType_capBits_def is_aligned_mask
-                       ARM_H.toAPIType_def ARM_H.toAPIType_def
+      apply (simp add: APIType_capBits_def is_aligned_mask toAPIType_def
                 split: ARM_H.object_type.splits)
      apply (simp add: vs_entry_align_def)
    apply (simp add: objBits_simps')
@@ -1169,7 +1198,7 @@ lemma createObject_valid_duplicates'[wp]:
                  word_bits_conv archObjSize_def is_aligned_mask
           split: ARM_H.object_type.splits)+)[1]
   apply (clarsimp simp: word_bits_def)
- done
+ sorry
 
 
 crunch arch_inv[wp]: createNewObjects "\<lambda>s. P (armKSGlobalPD (ksArchState s))"
@@ -1303,10 +1332,10 @@ lemma valid_duplicates_deleteObjects_helper:
     apply simp
    apply (simp add:vs_ptr_align_def)
   apply simp
-  done
+  sorry
 
 lemma deleteObjects_valid_duplicates'[wp]:
-  notes blah[simp del] =  atLeastatMost_subset_iff atLeastLessThan_iff
+  notes [simp del] =  atLeastatMost_subset_iff atLeastLessThan_iff
           Int_atLeastAtMost atLeastatMost_empty_iff split_paired_Ex
           atLeastAtMost_iff
   shows
@@ -1342,11 +1371,12 @@ lemma resetUntypedCap_valid_duplicates'[wp]:
   apply (rule hoare_pre)
    apply (wp | simp add: unless_def)+
    apply (wp mapME_x_inv_wp preemptionPoint_inv | simp | wp (once) hoare_drop_imps)+
+  sorry (*
    apply (wp getSlotCap_wp)
   apply (clarsimp simp: cte_wp_at_ctes_of split del: if_split)
   apply (frule cte_wp_at_valid_objs_valid_cap'[OF ctes_of_cte_wpD], clarsimp+)
   apply (clarsimp simp add: isCap_simps valid_cap_simps' capAligned_def)
-  done
+  done *)
 
 lemma is_aligned_armKSGlobalPD:
   "valid_arch_state' s
@@ -1376,6 +1406,7 @@ lemma invokeUntyped_valid_duplicates[wp]:
   apply (rule hoare_pre)
    apply simp
    apply (wp add: updateFreeIndex_pspace_no_overlap')
+  sorry (*
    apply (rule hoare_post_impErr)
      apply (rule combine_validE)
       apply (rule_tac ui=ui in whenE_reset_resetUntypedCap_invs_etc)
@@ -1395,7 +1426,7 @@ lemma invokeUntyped_valid_duplicates[wp]:
   apply (frule cte_wp_at_valid_objs_valid_cap'[OF ctes_of_cte_wpD], clarsimp+)
   apply (clarsimp simp add: isCap_simps valid_cap_simps' capAligned_def)
   apply (auto split: if_split_asm)
-  done
+  done *)
 
 crunch valid_duplicates'[wp]:
   doReplyTransfer "\<lambda>s. vs_valid_duplicates' (ksPSpace s)"
@@ -1439,7 +1470,7 @@ lemma set_asid_pool_valid_duplicates'[wp]:
 
 crunch valid_duplicates'[wp]:
   suspend "\<lambda>s. vs_valid_duplicates' (ksPSpace s)"
-  (wp: crunch_wps simp: crunch_simps unless_def o_def)
+  (wp: crunch_wps gts_wp' simp: crunch_simps unless_def o_def)
 
 crunch valid_duplicates'[wp]:
 deletingIRQHandler  "\<lambda>s. vs_valid_duplicates' (ksPSpace s)"
@@ -1554,18 +1585,14 @@ crunch valid_duplicates'[wp]:
  flushPage "\<lambda>s. vs_valid_duplicates' (ksPSpace s)"
   (wp: crunch_wps simp: crunch_simps unless_def)
 
-crunch valid_duplicates'[wp]:
- findPDForASID "\<lambda>s. vs_valid_duplicates' (ksPSpace s)"
-  (wp: crunch_wps simp: crunch_simps unless_def)
-
 lemma lookupPTSlot_aligned:
-  "\<lbrace>\<lambda>s. valid_objs' s \<and> vmsz_aligned' vptr sz \<and> sz \<noteq> ARMSuperSection\<rbrace>
+  "\<lbrace>\<lambda>s. valid_objs' s \<and> vmsz_aligned vptr sz \<and> sz \<noteq> ARMSuperSection\<rbrace>
    lookupPTSlot pd vptr
   \<lbrace>\<lambda>rv s. is_aligned rv ((pageBitsForSize sz) - 10)\<rbrace>,-"
   apply (simp add:lookupPTSlot_def)
   apply (wp|wpc|simp)+
   apply (wp getPDE_wp)
-  apply (clarsimp simp:obj_at'_def vmsz_aligned'_def)
+  apply (clarsimp simp:obj_at'_def vmsz_aligned_def)
   apply (clarsimp simp:projectKO_def fail_def
     projectKO_opt_pde return_def lookup_pt_slot_no_fail_def
     split:option.splits Structures_H.kernel_object.splits
@@ -1594,7 +1621,7 @@ crunch valid_arch_state'[wp]:
 lemma unmapPage_valid_duplicates'[wp]:
   notes checkMappingPPtr_inv[wp del] shows
   "\<lbrace>pspace_aligned' and valid_objs' and (\<lambda>s. vs_valid_duplicates' (ksPSpace s))
-   and K (vmsz_aligned' vptr vmpage_size)\<rbrace>
+   and K (vmsz_aligned vptr vmpage_size)\<rbrace>
   unmapPage vmpage_size asiv vptr word \<lbrace>\<lambda>r s. vs_valid_duplicates' (ksPSpace s)\<rbrace>"
   apply (simp add:unmapPage_def)
    (* make sure checkMappingPPtr_SmallPage is first tried before checkMappingPPtr_inv *)
@@ -1626,10 +1653,10 @@ lemma unmapPage_valid_duplicates'[wp]:
    apply (clarsimp simp:conj_comms)
    apply (rule hoare_post_imp_R[where Q'= "\<lambda>r. pspace_aligned' and
      (\<lambda>s. vs_valid_duplicates' (ksPSpace s)) and
-     K(vmsz_aligned' vptr vmpage_size \<and> is_aligned r pdBits)
+     K(vmsz_aligned vptr vmpage_size \<and> is_aligned r pdBits)
      and page_directory_at' (lookup_pd_slot r vptr && ~~ mask pdBits)"])
     apply (wp findPDForASID_page_directory_at' | simp)+
-   apply (clarsimp simp add:pdBits_def pageBits_def vmsz_aligned'_def)
+   apply (clarsimp simp add:pdBits_def pageBits_def vmsz_aligned_def)
    apply (drule is_aligned_lookup_pd_slot)
     apply (erule is_aligned_weaken,simp)
    apply simp
@@ -1674,7 +1701,8 @@ crunch valid_duplicates'[wp]:
  deleteASID "\<lambda>s. vs_valid_duplicates' (ksPSpace s)"
   (wp: crunch_wps simp: crunch_simps unless_def)
 
-crunches deleteASIDPool, unbindNotification, prepareThreadDelete
+crunches deleteASIDPool, unbindNotification, prepareThreadDelete, schedContextUnbindTCB,
+         schedContextCompleteYieldTo, schedContextUnbindAllTCBs
   for valid_duplicates'[wp]: "\<lambda>s. vs_valid_duplicates' (ksPSpace s)"
   (wp: crunch_wps simp: crunch_simps unless_def)
 
@@ -1692,8 +1720,10 @@ lemma finaliseCap_valid_duplicates'[wp]:
   "\<lbrace>valid_objs' and pspace_aligned' and (\<lambda>s. vs_valid_duplicates' (ksPSpace s))
   and (valid_cap' cap)\<rbrace>
   finaliseCap cap call final \<lbrace>\<lambda>r s. vs_valid_duplicates' (ksPSpace s)\<rbrace>"
-  apply (case_tac cap,simp_all add:isCap_simps finaliseCap_def)
-            apply (wp|intro conjI|clarsimp split: option.splits)+
+  apply (cases cap; simp add: isCap_simps finaliseCap_def)
+               apply (wpsimp wp: crunch_wps hoare_vcg_all_lift
+                             simp: crunch_simps split: option.splits
+                      | rule conjI)+
   done
 
 crunch valid_duplicates'[wp]:
@@ -1768,12 +1798,10 @@ lemma mapM_x_storePTE_invalid_whole:
   mapM_x (swp storePTE ARM_H.pte.InvalidPTE)
   [word , word + 2 ^ pteBits .e. word + 2 ^ ptBits - 1]
   \<lbrace>\<lambda>y s. vs_valid_duplicates' (ksPSpace s)\<rbrace>"
-  apply (wp mapM_x_storePTE_update_helper
-    [where word = word and sz = ptBits and ptr = word])
-  apply (clarsimp simp:valid_cap'_def capAligned_def pageBits_def
-    ptBits_def is_aligned_neg_mask_eq objBits_simps
-    archObjSize_def pteBits_def)
-  apply (simp add:mask_def field_simps pteBits_def)
+  apply (wp mapM_x_storePTE_update_helper[where word = word and sz = ptBits and ptr = word])
+  apply (clarsimp simp: valid_cap'_def capAligned_def pageBits_def ptBits_def objBits_simps
+                        archObjSize_def pteBits_def)
+  apply (simp add: mask_def field_simps pteBits_def)
   done
 
 crunch valid_objs'[wp]:
@@ -1784,24 +1812,18 @@ crunch pspace_aligned'[wp]:
   invalidateTLBByASID pspace_aligned'
   (wp: crunch_wps simp: crunch_simps unless_def)
 
-crunch valid_duplicates'[wp]:
-  isFinalCapability "\<lambda>s. vs_valid_duplicates' (ksPSpace s)"
-  (wp: crunch_wps filterM_preserved simp: crunch_simps unless_def)
-
 crunch valid_cap'[wp]:
   isFinalCapability "\<lambda>s. valid_cap' cap s"
   (wp: crunch_wps filterM_preserved simp: crunch_simps unless_def)
 
 crunch valid_duplicates'[wp]:
   sendSignal "\<lambda>s. vs_valid_duplicates' (ksPSpace s)"
+  (wp: crunch_wps simp: crunch_simps)
 
 lemma invokeIRQControl_valid_duplicates'[wp]:
   "\<lbrace>\<lambda>s. vs_valid_duplicates' (ksPSpace s) \<rbrace> performIRQControl a
-  \<lbrace>\<lambda>_ s. vs_valid_duplicates' (ksPSpace s)\<rbrace>"
-  apply (simp add:performIRQControl_def )
-  apply (rule hoare_pre)
-  apply (wp|wpc | simp add:ARM_H.performIRQControl_def)+
- done
+   \<lbrace>\<lambda>_ s. vs_valid_duplicates' (ksPSpace s)\<rbrace>"
+  unfolding performIRQControl_def by (wpsimp simp: ARM_H.performIRQControl_def)
 
 lemma invokeIRQHandler_valid_duplicates'[wp]:
   "\<lbrace>\<lambda>s. vs_valid_duplicates' (ksPSpace s) \<rbrace> invokeIRQHandler a
@@ -1825,14 +1847,8 @@ lemma invokeCNode_valid_duplicates'[wp]:
     apply (rule hoare_pre)
     apply (wp hoare_unless_wp | wpc | simp)+
    apply (simp add:invokeCNode_def)
-   apply (wp getSlotCap_inv hoare_drop_imp
-     |simp add:locateSlot_conv getThreadCallerSlot_def
-     |wpc)+
   apply (simp add:cteDelete_def invokeCNode_def)
-  apply (wp getSlotCap_inv hoare_drop_imp
-     |simp add:locateSlot_conv getThreadCallerSlot_def
-    whenE_def split_def
-     |wpc)+
+  apply (wp getSlotCap_inv hoare_drop_imp | simp add:locateSlot_conv whenE_def split_def | wpc)+
   apply (rule valid_validE)
    apply (rule hoare_post_imp[OF _ finaliseSlot_valid_duplicates'])
    apply simp
@@ -1949,14 +1965,12 @@ lemma placeASIDPool_valid_duplicates'[wp]:
      arch_kernel_object.splits Structures_H.kernel_object.splits )
      apply (drule mask_out_first_mask_some[where m = 12])
       apply simp
-     apply (clarsimp simp:mask_lower_twice field_simps
-       is_aligned_neg_mask_eq blah word_and_le2)
+     apply (clarsimp simp:mask_lower_twice field_simps blah word_and_le2)
      apply (rule order_trans[OF and_neg_mask_plus_mask_mono[where n = 12]])
      apply (simp add:mask_def)
     apply (drule mask_out_first_mask_some[where m = 12])
      apply simp
-    apply (clarsimp simp:mask_lower_twice field_simps
-      is_aligned_neg_mask_eq blah word_and_le2)
+    apply (clarsimp simp:mask_lower_twice field_simps blah word_and_le2)
     apply (rule order_trans[OF and_neg_mask_plus_mask_mono[where n = 12]])
     apply (simp add:mask_def)
    apply (simp add:obj_range'_def blah)
@@ -2036,25 +2050,72 @@ crunches restart
 crunches setPriority, setMCPriority
   for valid_duplicates'[wp]: "(\<lambda>s. vs_valid_duplicates' (ksPSpace s))"
   (ignore: threadSet
-       wp: setObject_ksInterrupt updateObject_default_inv
+       wp: setObject_ksInterrupt updateObject_default_inv crunch_wps
      simp: crunch_simps)
 
-crunch inv[wp]: getThreadBufferSlot P
-  (wp: crunch_wps)
+crunches installFaultHandler, installThreadBuffer, installVRoot, installCRoot,
+         installTimeoutHandler
+  for valid_duplicates'[wp]: "(\<lambda>s. vs_valid_duplicates' (ksPSpace s))"
+  (wp:  crunch_wps checkCap_inv
+   simp: crunch_simps getThreadVSpaceRoot_def getThreadFaultHandlerSlot_def
+         getThreadTimeoutHandlerSlot_def
+   ignore: checkCapAt)
 
-lemma tc_valid_duplicates':
-  "\<lbrace>invs' and sch_act_simple and (\<lambda>s. vs_valid_duplicates' (ksPSpace s)) and tcb_at' a and ex_nonz_cap_to' a and
-    case_option \<top> (valid_cap' o fst) e' and
-    K (case_option True (isCNodeCap o fst) e') and
-    case_option \<top> (valid_cap' o fst) f' and
-    K (case_option True (isValidVTableRoot o fst) f') and
-    case_option \<top> (valid_cap') (case_option None (case_option None (Some o fst) o snd) g) and
-    K (valid_option_prio d) and
-    K (valid_option_prio mcp) and
-    K (case_option True isArchObjectCap (case_option None (case_option None (Some o fst) o snd) g))
-    and K (case_option True (swp is_aligned msg_align_bits o fst) g)\<rbrace>
-      invokeTCB (tcbinvocation.ThreadControl a sl b' mcp d e' f' g)
+lemma tc_caps_valid_duplicates':
+  "\<lbrace>invs' and sch_act_simple and (\<lambda>s. vs_valid_duplicates' (ksPSpace s)) and
+    tcb_at' t and ex_nonz_cap_to' t and
+    case_option \<top> (valid_cap' o fst) croot and
+    K (case_option True (isCNodeCap o fst) croot) and
+    case_option \<top> (valid_cap' o fst) vroot and
+    K (case_option True (isValidVTableRoot o fst) vroot) and
+    case_option \<top> (valid_cap') (case_option None (case_option None (Some o fst) o snd) ipcb) and
+    K (case_option True isArchObjectCap (case_option None (case_option None (Some o fst) o snd) ipcb))
+    and K (case_option True (swp is_aligned msg_align_bits o fst) ipcb)\<rbrace>
+      invokeTCB (ThreadControlCaps t sl fault_h timout_h croot vroot ipcb)
    \<lbrace>\<lambda>rv s. vs_valid_duplicates' (ksPSpace s)\<rbrace>"
+  apply (simp add: split_def invokeTCB_def getThreadCSpaceRoot getThreadVSpaceRoot
+                   getThreadBufferSlot_def locateSlot_conv
+             cong: option.case_cong)
+  sorry (*
+  apply (simp only: eq_commute[where a="t"])
+  apply (rule hoare_walk_assmsE)
+    apply (clarsimp simp: pred_conj_def option.splits [where P="\<lambda>x. x s" for s])
+    apply ((wp case_option_wp threadSet_invs_trivial static_imp_wp
+               hoare_vcg_all_lift threadSet_cap_to' | clarsimp simp: inQ_def)+)[2]
+  apply (rule hoare_walk_assmsE)
+    apply (clarsimp simp: pred_conj_def option.splits [where P="\<lambda>x. x s" for s])
+    apply ((wp case_option_wp threadSet_invs_trivial static_imp_wp setMCPriority_invs'
+               typ_at_lifts[OF setMCPriority_typ_at']
+               hoare_vcg_all_lift threadSet_cap_to' | clarsimp simp: inQ_def)+)[2]
+  apply ((simp only: simp_thms cases_simp cong: conj_cong
+          | (wp cteDelete_deletes cteDelete_invs' cteDelete_sch_act_simple
+              threadSet_ipcbuffer_trivial
+              (* setPriority has no effect on vs_duplicates *)
+              case_option_wp[where m'="return ()", OF setPriority_valid_duplicates' return_inv,simplified]
+              checkCap_inv[where P="tcb_at' t" for t]
+              checkCap_inv[where P="valid_cap' c" for c]
+              checkCap_inv[where P="\<lambda>s. P (ksReadyQueues s)" for P]
+              checkCap_inv[where P="\<lambda>s. vs_valid_duplicates' (ksPSpace s)"]
+              checkCap_inv[where P=sch_act_simple] cteDelete_valid_duplicates' hoare_vcg_const_imp_lift_R
+              typ_at_lifts[OF setPriority_typ_at'] assertDerived_wp threadSet_cte_wp_at'
+              hoare_vcg_all_lift_R hoare_vcg_all_lift static_imp_wp)[1]
+          | wpc
+          | simp add: inQ_def
+          | wp hoare_vcg_conj_liftE1 cteDelete_invs' cteDelete_deletes hoare_vcg_const_imp_lift)+)
+  apply (clarsimp simp: tcb_cte_cases_def cte_level_bits_def objBits_defs
+                        tcbIPCBufferSlot_def)
+  by (auto dest!: isCapDs isReplyCapD isValidVTableRootD simp: isCap_simps)
+  *)
+
+lemma tc_sched_valid_duplicates':
+  "\<lbrace>invs' and sch_act_simple and (\<lambda>s. vs_valid_duplicates' (ksPSpace s)) and
+    tcb_at' t and ex_nonz_cap_to' t and
+    case_option \<top> (valid_cap' o fst) sc_fh and
+    K (valid_option_prio pri) and
+    K (valid_option_prio mcp)\<rbrace>
+      invokeTCB  (ThreadControlSched t sl sc_fh pri mcp sc_opt)
+   \<lbrace>\<lambda>rv s. vs_valid_duplicates' (ksPSpace s)\<rbrace>"
+  sorry (*
   apply (rule hoare_gen_asm)
   apply (simp add: split_def invokeTCB_def getThreadCSpaceRoot getThreadVSpaceRoot
                    getThreadBufferSlot_def locateSlot_conv
@@ -2087,6 +2148,7 @@ lemma tc_valid_duplicates':
   apply (clarsimp simp: tcb_cte_cases_def cte_level_bits_def objBits_defs
                         tcbIPCBufferSlot_def)
   by (auto dest!: isCapDs isReplyCapD isValidVTableRootD simp: isCap_simps)
+ *)
 
 crunches performTransfer, unbindNotification, bindNotification, setDomain
   for valid_duplicates'[wp]: "(\<lambda>s. vs_valid_duplicates' (ksPSpace s))"
@@ -2098,27 +2160,29 @@ lemma invokeTCB_valid_duplicates'[wp]:
   "\<lbrace>invs' and sch_act_simple and ct_in_state' runnable' and tcb_inv_wf' ti and (\<lambda>s. vs_valid_duplicates' (ksPSpace s))\<rbrace>
      invokeTCB ti
    \<lbrace>\<lambda>rv s. vs_valid_duplicates' (ksPSpace s)\<rbrace>"
-  apply (case_tac ti, simp_all only:)
-       apply (simp add: invokeTCB_def)
-       apply wp
-       apply (clarsimp simp: invs'_def valid_state'_def
-                      dest!: global'_no_ex_cap)
-      apply (simp add: invokeTCB_def)
-      apply wp
-      apply (clarsimp simp: invs'_def valid_state'_def
-                     dest!: global'_no_ex_cap)
-     apply (wp tc_valid_duplicates')
-     apply (clarsimp split:option.splits)
-     apply (rename_tac option)
-     apply (case_tac option, simp_all)
-    apply (simp add:invokeTCB_def | wp mapM_x_wp' | intro impI conjI | wpc)+
+  apply (case_tac ti; simp only:)
+          apply (simp add: invokeTCB_def)
+          apply wp
+          apply (clarsimp simp: invs'_def valid_state'_def
+                         dest!: global'_no_ex_cap)
+         apply (simp add: invokeTCB_def)
+         apply wp
+         apply (clarsimp simp: invs'_def valid_state'_def
+                        dest!: global'_no_ex_cap)
+        apply (wpsimp wp: tc_caps_valid_duplicates' split: option.splits)
+       apply (wpsimp wp: tc_sched_valid_duplicates')
+      apply (simp add:invokeTCB_def | wp mapM_x_wp' | intro impI conjI | wpc)+
   done
+
+crunches invokeSchedContext, invokeSchedControlConfigure
+  for valid_duplicates'[wp]: "\<lambda>s. vs_valid_duplicates' (ksPSpace s)"
+  (simp: crunch_simps wp: crunch_wps hoare_vcg_all_lift)
 
 lemma performInvocation_valid_duplicates'[wp]:
   "\<lbrace>\<lambda>s. vs_valid_duplicates' (ksPSpace s) \<and> invs' s \<and> sch_act_simple s
     \<and> valid_invocation' i s \<and> ct_active' s\<rbrace>
-  RetypeDecls_H.performInvocation isBlocking isCall i
-  \<lbrace>\<lambda>reply s. vs_valid_duplicates' (ksPSpace s)\<rbrace>"
+  RetypeDecls_H.performInvocation isBlocking isCall canDonate i
+  \<lbrace>\<lambda>_ s. vs_valid_duplicates' (ksPSpace s)\<rbrace>"
   apply (clarsimp simp:performInvocation_def)
   apply (simp add:ct_in_state'_def)
   apply (rule hoare_name_pre_state)
@@ -2136,7 +2200,7 @@ lemma performInvocation_valid_duplicates'[wp]:
 lemma hi_valid_duplicates'[wp]:
   "\<lbrace>invs' and sch_act_simple and ct_active'
     and (\<lambda>s. vs_valid_duplicates' (ksPSpace s))\<rbrace>
-      handleInvocation isCall isBlocking
+      handleInvocation isCall isBlocking canDonate firstPhase cptr
    \<lbrace>\<lambda>r s. vs_valid_duplicates' (ksPSpace s) \<rbrace>"
   apply (simp add: handleInvocation_def split_def
                    ts_Restart_case_helper')
@@ -2149,20 +2213,9 @@ lemma hi_valid_duplicates'[wp]:
                         dest: st_tcb_at_idle_thread')+
   done
 
-crunch valid_duplicates' [wp]:
-  activateIdleThread "(\<lambda>s. vs_valid_duplicates' (ksPSpace s))"
+crunches activateIdleThread, schedContextCompleteYieldTo
+  for valid_duplicates' [wp]: "\<lambda>s. vs_valid_duplicates' (ksPSpace s)"
   (ignore: setNextPC threadSet simp:crunch_simps)
-
-crunch valid_duplicates' [wp]:
-  tcbSchedAppend "(\<lambda>s. vs_valid_duplicates' (ksPSpace s))"
-  (simp:crunch_simps wp:hoare_unless_wp)
-
-lemma timerTick_valid_duplicates'[wp]:
-  "\<lbrace>\<lambda>s. vs_valid_duplicates' (ksPSpace s)\<rbrace>
-  timerTick \<lbrace>\<lambda>x s. vs_valid_duplicates' (ksPSpace s)\<rbrace>"
-  apply (simp add:timerTick_def decDomainTime_def)
-   apply (wp hoare_drop_imps|wpc|simp)+
-  done
 
 lemma handleInterrupt_valid_duplicates'[wp]:
   "\<lbrace>\<lambda>s. vs_valid_duplicates' (ksPSpace s)\<rbrace>
@@ -2174,10 +2227,10 @@ lemma handleInterrupt_valid_duplicates'[wp]:
           |wpc|simp add: handleReservedIRQ_def)+
   done
 
-
 crunch valid_duplicates' [wp]:
-  schedule "(\<lambda>s. vs_valid_duplicates' (ksPSpace s))"
-  (ignore: setNextPC clearExMonitor threadSet simp:crunch_simps wp:findM_inv hoare_drop_imps)
+  schedule "\<lambda>s. vs_valid_duplicates' (ksPSpace s)"
+  (ignore: setNextPC clearExMonitor threadSet simp: crunch_simps
+   wp: whileM_inv findM_inv hoare_drop_imps)
 
 lemma activate_sch_valid_duplicates'[wp]:
   "\<lbrace>\<lambda>s. ct_in_state' activatable' s \<and> vs_valid_duplicates' (ksPSpace s)\<rbrace>
@@ -2185,41 +2238,24 @@ lemma activate_sch_valid_duplicates'[wp]:
   apply (simp add: activateThread_def getCurThread_def
              cong: if_cong Structures_H.thread_state.case_cong)
   apply (rule hoare_seq_ext [OF _ gets_sp])
-  apply (rule hoare_seq_ext[where B="\<lambda>st s.  (runnable' or idle') st
-    \<and> vs_valid_duplicates' (ksPSpace s)"])
-   apply (rule hoare_pre)
-    apply (wp | wpc | simp add: setThreadState_runnable_simp)+
-  apply (clarsimp simp: ct_in_state'_def cur_tcb'_def pred_tcb_at'
-                 elim!: pred_tcb'_weakenE)
+  apply (rule hoare_seq_ext[where B="\<lambda>st s. (runnable' or idle') st \<and>
+                                            vs_valid_duplicates' (ksPSpace s)"])
+   apply (wpsimp wp: threadGet_wp hoare_drop_imps)
+   apply (clarsimp simp: obj_at'_def)
+  apply (wp gts_wp')
+  apply (clarsimp simp: pred_tcb_at'_def ct_in_state'_def obj_at'_def)
   done
 
-crunch valid_duplicates'[wp]:
-  receiveSignal "\<lambda>s. vs_valid_duplicates' (ksPSpace s)"
-
-crunch valid_duplicates'[wp]:
-  receiveIPC "\<lambda>s. vs_valid_duplicates' (ksPSpace s)"
-(wp: getNotification_wp gbn_wp')
-
-crunch valid_duplicates'[wp]:
-  deleteCallerCap "\<lambda>s. vs_valid_duplicates' (ksPSpace s)"
+crunches receiveSignal, receiveIPC, handleYield, "VSpace_H.handleVMFault", handleHypervisorFault,
+         lookupReply, checkBudgetRestart
+  for valid_duplicates'[wp]: "\<lambda>s. vs_valid_duplicates' (ksPSpace s)"
   (wp: crunch_wps)
-
-crunch valid_duplicates'[wp]:
-  handleReply "\<lambda>s. vs_valid_duplicates' (ksPSpace s)"
-
-crunch valid_duplicates'[wp]:
-  handleYield "\<lambda>s. vs_valid_duplicates' (ksPSpace s)"
- (ignore: threadGet simp:crunch_simps wp:hoare_unless_wp)
-
-crunch valid_duplicates'[wp]:
-  "VSpace_H.handleVMFault", handleHypervisorFault "\<lambda>s. vs_valid_duplicates' (ksPSpace s)"
- (ignore: getFAR getDFSR getIFSR simp:crunch_simps)
 
 lemma hs_valid_duplicates'[wp]:
   "\<lbrace>invs' and ct_active' and sch_act_simple and (\<lambda>s. vs_valid_duplicates' (ksPSpace s))\<rbrace>
   handleSend blocking \<lbrace>\<lambda>r s. vs_valid_duplicates' (ksPSpace s)\<rbrace>"
   apply (rule validE_valid)
-  apply (simp add: handleSend_def)
+  apply (simp add: handleSend_def getCapReg_def)
   apply (wp | simp)+
   done
 
@@ -2227,23 +2263,19 @@ lemma hc_valid_duplicates'[wp]:
   "\<lbrace>invs' and ct_active' and sch_act_simple and (\<lambda>s. vs_valid_duplicates' (ksPSpace s))\<rbrace>
      handleCall
    \<lbrace>\<lambda>rv s. vs_valid_duplicates' (ksPSpace s)\<rbrace>"
-  by (simp add: handleCall_def |  wp)+
+  by (simp add: handleCall_def getCapReg_def | wp)+
 
 lemma handleRecv_valid_duplicates'[wp]:
   "\<lbrace>(\<lambda>s. vs_valid_duplicates' (ksPSpace s))\<rbrace>
-  handleRecv isBlocking \<lbrace>\<lambda>r s. vs_valid_duplicates' (ksPSpace s)\<rbrace>"
-  apply (simp add: handleRecv_def cong: if_cong)
+  handleRecv isBlocking canDonate \<lbrace>\<lambda>r s. vs_valid_duplicates' (ksPSpace s)\<rbrace>"
+  apply (simp add: handleRecv_def cong: if_cong split del: if_split)
   apply (rule hoare_pre)
    apply wp
-       apply ((wp getNotification_wp | wpc | simp add: whenE_def split del: if_split)+)[1]
-
-      apply (rule_tac Q="\<lambda>rv s. vs_valid_duplicates' (ksPSpace s)"
-
-                   in hoare_post_impErr[rotated])
-
-        apply (clarsimp simp: isCap_simps sch_act_sane_not)
-       apply assumption
-      apply (wp deleteCallerCap_nonz_cap)+
+      apply ((wp getNotification_wp | wpc | simp add: whenE_def split del: if_split)+)[1]
+     apply (rule_tac Q="\<lambda>rv s. vs_valid_duplicates' (ksPSpace s)" in hoare_post_impErr[rotated])
+       apply (clarsimp simp: isCap_simps sch_act_sane_not)
+      apply assumption
+     apply (wp)+
   apply (auto elim: st_tcb_ex_cap'' pred_tcb'_weakenE
              dest!: st_tcb_at_idle_thread'
               simp: ct_in_state'_def sch_act_sane_def)
@@ -2255,13 +2287,14 @@ lemma handleEvent_valid_duplicates':
     sch_act_simple and (\<lambda>s. e \<noteq> Interrupt \<longrightarrow> ct_running' s)\<rbrace>
    handleEvent e
    \<lbrace>\<lambda>rv s. vs_valid_duplicates' (ksPSpace s)\<rbrace>"
-  apply (case_tac e, simp_all add: handleEvent_def)
-      apply (rename_tac syscall)
-      apply (case_tac syscall)
-            apply (wp handleReply_sane
-              | simp add: active_from_running' simple_sane_strg cong: if_cong
-              | wpc)+
-  done
+  apply (case_tac e; simp add: handleEvent_def)
+       apply (rename_tac syscall)
+       apply (case_tac syscall)
+  sorry (*
+                 apply (wp
+                   | simp add: active_from_running' simple_sane_strg cong: if_cong
+                   | wpc)+
+  done *)
 
 lemma callKernel_valid_duplicates':
   "\<lbrace>invs' and (\<lambda>s. vs_valid_duplicates' (ksPSpace s)) and
@@ -2271,9 +2304,10 @@ lemma callKernel_valid_duplicates':
    \<lbrace>\<lambda>rv s. vs_valid_duplicates' (ksPSpace s)\<rbrace>"
   apply (simp add: callKernel_def)
   apply (rule hoare_pre)
-   apply (wp activate_invs' activate_sch_act schedule_sch
+   apply (wp activate_invs'  schedule_sch
              schedule_sch_act_simple he_invs'
           | simp add: no_irq_getActiveIRQ)+
+  sorry (* mcsIRQ
    apply (rule hoare_post_impErr)
      apply (rule valid_validE)
      prefer 2
@@ -2281,7 +2315,7 @@ lemma callKernel_valid_duplicates':
     apply (wp handleEvent_valid_duplicates')
    apply simp
   apply simp
-  done
+  done *)
 
 end
 
